start work on information flow semantics

theories/caesium/val.v
@@ -1,23 +1,26 @@
-From caesium Require Export base byte layout int_type loc struct.
+From caesium Require Export base byte layout int_type loc struct security.
 Set Default Proof Using "Type".
 
 (** * Bytes and values stored in memory *)
+Section vals.
+Context `{!ConfidentialInterface}.
 
 (** Representation of a byte stored in memory. *)
 Inductive mbyte : Set :=
-| MByte (b : byte) (p : option alloc_id) (** [p] is Some if this integer contains provenance *)
-| MPtrFrag (l : loc) (n : nat) (** Fragment [n] for location [l]. *)
+| MByte (b : byte) (p : option alloc_id) (α : slevel) (** [p] is Some if this integer contains provenance *)
+| MPtrFrag (l : loc) (n : nat) (α : slevel) (** Fragment [n] for location [l]. *)
 | MPoison.
 
 #[export] Instance mbyte_dec_eq : EqDecision mbyte.
 Proof. solve_decision. Qed.
 
-Program Definition mbyte_to_byte (mb : mbyte) : option (byte * option alloc_id) :=
+Program Definition mbyte_to_byte (mb : mbyte) : option (byte * option alloc_id * slevel) :=
   match mb with
-  | MByte b p => Some (b, p)
-  | MPtrFrag l n => Some (
+  | MByte b p α => Some (b, p, α)
+  | MPtrFrag l n α => Some (
      {| byte_val := ((l.2 `div` 2^(8 * n)) `mod` byte_modulus) |},
-     if l.1 is ProvAlloc a then a else None)
+     if l.1 is ProvAlloc a then a else None, 
+     α)
   | MPoison => None
   end.
 Next Obligation. move => ? l n. have [] := Z_mod_lt (l.2 `div` 2 ^ (8 * n)) byte_modulus => //*. lia. Qed.
@@ -35,72 +38,84 @@ Notation "v `has_layout_val` n" := (has_layout_val v n) (at level 50) : stdpp_sc
 Arguments has_layout_val : simpl never.
 Global Typeclasses Opaque has_layout_val.
 
+(** Predicate stating that a byte is at most as secure as α *)
+(* TODO: Is poison secure? Can I get information leakage by observing whether it is UB or not? 
+  For now, I assume that poison has any security level.
+  I think this is okay because our final theorem will assume that the execution is safe. *)
+Definition has_security_mbyte (mb : mbyte) (α : slevel) :=
+  match mbyte_to_byte mb with
+  | None => True
+  | Some (_, _, α') => α' ⊑ α
+  end.
+Definition has_security_val (v : val) (α : slevel) :=
+  Forall (λ mb, has_security_mbyte mb α) v.
+
 (** ** Conversion to and from locations. *)
 (* rev because we do little endian *)
-Definition val_of_loc_n (n : nat) (l : loc) : val :=
-  MPtrFrag l <$> rev (seq 0 n).
+Definition val_of_loc_n (n : nat) (α : slevel) (l : loc) : val :=
+  (λ n, MPtrFrag l n α) <$> rev (seq 0 n).
 
-Definition val_of_loc : loc → val :=
+Definition val_of_loc : slevel → loc → val :=
   val_of_loc_n bytes_per_addr.
 
 (* [NULL_bytes(_n)] is the alternative representation of NULL as integer 0 bytes. *)
-Definition NULL_bytes_n (n : nat) : val := repeat (MByte byte0 None) n.
-Definition NULL_bytes := NULL_bytes_n bytes_per_addr.
+Definition NULL_bytes_n (α : slevel) (n : nat) : val := repeat (MByte byte0 None α) n.
+Definition NULL_bytes (α : slevel) := NULL_bytes_n α bytes_per_addr.
 
-Definition val_to_loc_n (n : nat) (v : val) : option loc :=
-  if v is MPtrFrag l _ :: _ then
-    if (bool_decide (v = val_of_loc_n n l)) then Some l else None
+Definition val_to_loc_n (n : nat) (v : val) : option (slevel * loc) :=
+  if v is MPtrFrag l _ α :: _ then
+    if (bool_decide (v = val_of_loc_n n α l)) then Some (α, l) else None
   (* A list of 0s is interpreted as NULL. This is mainly useful when
   memcasting is turned off. Interpreting 0s as NULL does not cause the
   steps for pointers to overlap with the steps for integers since the
   steps are dispatched based on the op_type, not on val_to_loc. *)
-  else if v is MByte b _ :: _ then
-    if (bool_decide (v = NULL_bytes_n n)) then Some NULL_loc else None
+  else if v is MByte b _ α :: _ then
+    if (bool_decide (v = NULL_bytes_n α n)) then Some (α, NULL_loc) else None
   else None.
 
-Definition val_to_loc : val → option loc :=
+Definition val_to_loc : val → option (slevel * loc) :=
   val_to_loc_n bytes_per_addr.
 
-Definition NULL : val := val_of_loc NULL_loc.
+Definition NULL : val := val_of_loc ⊥ NULL_loc.
 Global Typeclasses Opaque NULL.
 
-Lemma val_of_loc_n_length n l:
-  length (val_of_loc_n n l) = n.
+Lemma val_of_loc_n_length α n l:
+  length (val_of_loc_n n α l) = n.
 Proof.
   by rewrite /val_of_loc_n fmap_length rev_length seq_length.
 Qed.
 
-Lemma val_to_of_loc_n n l:
+Lemma val_to_of_loc_n α n l:
   n ≠ 0%nat →
-  val_to_loc_n n (val_of_loc_n n l) = Some l.
+  val_to_loc_n n (val_of_loc_n n α l) = Some (α, l).
 Proof.
   destruct n as [|n]; first done.
   rewrite /val_of_loc_n seq_S rev_unit /= bool_decide_true //.
   by rewrite /val_of_loc_n seq_S rev_unit.
 Qed.
 
-Lemma val_to_of_loc l:
-  val_to_loc (val_of_loc l) = Some l.
+Lemma val_to_of_loc α l:
+  val_to_loc (val_of_loc α l) = Some (α, l).
 Proof.
   by apply val_to_of_loc_n.
 Qed.
 
-Lemma val_of_to_loc_n n v l:
-  val_to_loc_n n v = Some l → v = val_of_loc_n n l ∨ v = NULL_bytes_n n ∧ l = NULL_loc.
+Lemma val_of_to_loc_n α n v l:
+  val_to_loc_n n v = Some (α, l) → v = val_of_loc_n n α l ∨ v = NULL_bytes_n α n ∧ l = NULL_loc.
 Proof.
   rewrite /val_to_loc_n.
   destruct v as [|b v'] eqn:Hv; first done.
   repeat case_match => //; case_bool_decide; naive_solver.
 Qed.
 
-Lemma val_of_to_loc v l:
-  val_to_loc v = Some l → v = val_of_loc l ∨ v = NULL_bytes ∧ l = NULL_loc.
+Lemma val_of_to_loc α v l:
+  val_to_loc v = Some (α, l) → v = val_of_loc α l ∨ v = NULL_bytes α ∧ l = NULL_loc.
 Proof. apply val_of_to_loc_n. Qed.
 
 Lemma val_to_loc_n_length n v:
   is_Some (val_to_loc_n n v) → length v = n.
 Proof.
-  rewrite /val_to_loc_n. move => [? H]. repeat case_match => //; simplify_eq.
+  rewrite /val_to_loc_n. move => [? Hs]. repeat case_match => //; simplify_eq.
   - revert select (bool_decide _ = _) => /bool_decide_eq_true ->.
     rewrite /NULL_bytes_n. by rewrite repeat_length.
   - revert select (bool_decide _ = _) => /bool_decide_eq_true ->.
@@ -111,8 +126,8 @@ Lemma val_to_loc_length v:
   is_Some (val_to_loc v) → length v = bytes_per_addr.
 Proof. apply val_to_loc_n_length. Qed.
 
-Global Instance val_of_loc_inj : Inj (=) (=) val_of_loc.
-Proof. move => x y Heq. have := val_to_of_loc x. have := val_to_of_loc y. rewrite Heq. by simplify_eq. Qed.
+Global Instance val_of_loc_inj : Inj2 (=) (=) (=) val_of_loc.
+Proof. move => α1 x α2 y Heq. have := val_to_of_loc α1 x. have := val_to_of_loc α2 y. rewrite Heq. by simplify_eq. Qed.
 
 Global Typeclasses Opaque val_of_loc_n val_to_loc_n val_of_loc val_to_loc.
 Arguments val_of_loc : simpl never.
@@ -126,75 +141,83 @@ Arguments val_to_loc : simpl never.
 
 (* TODO: we currently assume little-endian, make this more generic. *)
 
-Fixpoint val_to_Z_go v : option Z :=
+Fixpoint val_to_Z_go v : option (slevel * Z) :=
   match v with
-  | []           => Some 0
-  | MByte b _ :: v => z ← val_to_Z_go v; Some (byte_modulus * z + b.(byte_val))
+  | []           => Some (⊥, 0)
+  | MByte b _ α :: v => 
+      '(α', z) ← val_to_Z_go v;
+      Some (α ⊔ α', byte_modulus * z + b.(byte_val))
   | _            => None
   end.
 
-Definition val_to_Z (v : val) (it : int_type) : option Z :=
+Definition val_to_Z (v : val) (it : int_type) : option (slevel * Z) :=
   if bool_decide (length v = bytes_per_int it) then
-    z ← val_to_Z_go v;
+    '(α, z) ← val_to_Z_go v;
     if it.(it_signed) && bool_decide (int_half_modulus it ≤ z) then
-      Some (z - int_modulus it)
+      Some (α, z - int_modulus it)
     else
-      Some z
+      Some (α, z)
   else None.
 
 Definition val_to_byte_prov (v : val) : option alloc_id :=
-  if v is MByte _ (Some p) :: _ then
-    guard (Forall (λ e, Is_true (if e is MByte _ (Some p') then bool_decide (p = p') else false)) v); Some p
+  if v is MByte _ (Some p) _ :: _ then
+    guard (Forall (λ e, Is_true (if e is MByte _ (Some p') _ then bool_decide (p = p') else false)) v); Some p
   else None.
 
 Definition provs_in_bytes (v : val) : list alloc_id :=
-  omap (λ b, if b is MByte _ (Some p) then Some p else None) v.
+  omap (λ b, if b is MByte _ (Some p) _ then Some p else None) v.
 
 Definition val_to_bytes (v : val) : option val :=
-  mapM (λ b, (λ '(v, a), MByte v a) <$> mbyte_to_byte b) v.
+  mapM (λ b, (λ '(v, a, α), MByte v a α) <$> mbyte_to_byte b) v.
 
-Program Fixpoint val_of_Z_go (n : Z) (sz : nat) (p : option alloc_id) : val :=
+Program Fixpoint val_of_Z_go (n : Z) (sz : nat) (p : option alloc_id) (α : slevel) : val :=
   match sz return _ with
   | O    => []
-  | S sz => MByte {| byte_val := (n `mod` byte_modulus) |} p
-            :: val_of_Z_go (n / byte_modulus) sz p
+  | S sz => MByte {| byte_val := (n `mod` byte_modulus) |} p α
+            :: val_of_Z_go (n / byte_modulus) sz p α
   end.
 Next Obligation. move => n. have [] := Z_mod_lt n byte_modulus => //*. lia. Qed.
 
-Definition val_of_Z (z : Z) (it : int_type) (p : option alloc_id) : option val :=
+Definition val_of_Z (z : Z) (it : int_type) (p : option alloc_id) (α : slevel) : option val :=
   if bool_decide (z ∈ it) then
     let n := if bool_decide (z < 0) then z + int_modulus it else z in
-    Some (val_of_Z_go n (bytes_per_int it) p)
+    Some (val_of_Z_go n (bytes_per_int it) p α)
   else
     None.
 
-Definition i2v (n : Z) (it : int_type) : val :=
-  default (replicate (bytes_per_int it) MPoison) (val_of_Z n it None).
+Definition i2v (n : Z) (it : int_type) (α : slevel) : val :=
+  default (replicate (bytes_per_int it) MPoison) (val_of_Z n it None α).
 
-Lemma val_of_Z_go_length z sz p:
-  length (val_of_Z_go z sz p) = sz.
+Lemma val_of_Z_go_length z sz p α :
+  length (val_of_Z_go z sz p α) = sz.
 Proof. elim: sz z => //= ? IH ?. by f_equal. Qed.
 
-Lemma val_to_of_Z_go z (sz : nat) p:
+Lemma val_to_of_Z_go z (sz : nat) p α :
+  0 < sz →
   0 ≤ z < 2 ^ (sz * bits_per_byte) →
-  val_to_Z_go (val_of_Z_go z sz p) = Some z.
+  val_to_Z_go (val_of_Z_go z sz p α) = Some (α, z).
 Proof.
   rewrite /bits_per_byte.
-  elim: sz z => /=. 1: rewrite /Z.of_nat; move => ??; f_equal; lia.
-  move => sz IH z [? Hlt]. rewrite IH /byte_modulus /= -?Z_div_mod_eq_full //.
+  elim: sz z => /=. 1: rewrite /Z.of_nat; move => ???; f_equal; lia.
+  move => sz IH z Hnz [? Hlt]. 
+  destruct sz. { simpl in *. rewrite Z.mul_0_r Z.add_0_l.
+    rewrite/byte_modulus /=.
+    f_equiv. f_equiv. { rewrite slevel_bot_neutral_r//. } 
+    lia. }
+  rewrite IH /byte_modulus /= -?Z_div_mod_eq_full //.
+  { rewrite slevel_join_idemp//. } 
   split; [by apply Z_div_pos|]. apply Zdiv_lt_upper_bound => //.
   rewrite Nat2Z.inj_succ -Zmult_succ_l_reverse Z.pow_add_r // in Hlt.
-  lia.
 Qed.
 
-Lemma val_of_Z_length z it v p:
-  val_of_Z z it p = Some v → length v = bytes_per_int it.
+Lemma val_of_Z_length z it v p α :
+  val_of_Z z it p α = Some v → length v = bytes_per_int it.
 Proof.
   rewrite /val_of_Z => Hv. case_bool_decide => //. simplify_eq.
   by rewrite val_of_Z_go_length.
 Qed.
 
-Lemma i2v_length n it: length (i2v n it) = bytes_per_int it.
+Lemma i2v_length n it α : length (i2v n it α) = bytes_per_int it.
 Proof.
   rewrite /i2v. destruct (val_of_Z n it None) eqn:Heq.
   - by apply val_of_Z_length in Heq.
@@ -205,34 +228,34 @@ Lemma val_to_Z_length v it z:
   val_to_Z v it = Some z → length v = bytes_per_int it.
 Proof. rewrite /val_to_Z. by case_decide. Qed.
 
-Lemma val_of_Z_is_Some p it z:
-  z ∈ it → is_Some (val_of_Z z it p).
+Lemma val_of_Z_is_Some p it z α :
+  z ∈ it → is_Some (val_of_Z z it p α).
 Proof. rewrite /val_of_Z. case_bool_decide; by eauto. Qed.
 
-Lemma val_of_Z_in_range it z v p:
-  val_of_Z z it p = Some v → z ∈ it.
+Lemma val_of_Z_in_range it z v p α :
+  val_of_Z z it p α = Some v → z ∈ it.
 Proof. rewrite /val_of_Z. case_bool_decide; by eauto. Qed.
 
-Lemma val_to_Z_go_in_range v n:
-  val_to_Z_go v = Some n → 0 ≤ n < 2 ^ (length v * bits_per_byte).
+Lemma val_to_Z_go_in_range v n α :
+  val_to_Z_go v = Some (α, n) → 0 ≤ n < 2 ^ (length v * bits_per_byte).
 Proof.
-  elim: v n => /=.
-  - move => n [] <-. split; first lia.
+  elim: v n α => /=.
+  - move => n ? [] ? <-. split; first lia.
     apply Z.pow_pos_nonneg; lia.
-  - move => ? v IH n. case_match => //.
-    destruct (val_to_Z_go v) => /=; last done.
-    move => [] <-. move: (IH z eq_refl).
+  - move => ? v IH n α. case_match => //.
+    destruct (val_to_Z_go v) as [[] | ] => /=; last done.
+    move => [] ? <-. move: (IH z _ eq_refl).
     move: (byte_constr b). rewrite /byte_modulus /bits_per_byte.
     move => [??] [??]. split; first lia.
     have ->: S (length v) * 8 = 8 + length v * 8 by lia.
     rewrite Z.pow_add_r; lia.
 Qed.
 
-Lemma val_to_Z_in_range v it n:
-  val_to_Z v it = Some n → n ∈ it.
+Lemma val_to_Z_in_range v it n α :
+  val_to_Z v it = Some (α, n) → n ∈ it.
 Proof.
   rewrite /val_to_Z. case_decide as Hlen; last done.
-  destruct (val_to_Z_go v) eqn:Heq => /=; last done.
+  destruct (val_to_Z_go v) as [[] | ] eqn:Heq => /=; last done.
   move: Heq => /val_to_Z_go_in_range.
   rewrite Hlen /elem_of /int_elem_of_it /max_int /min_int.
   rewrite /int_half_modulus /int_modulus /bits_per_int.
@@ -248,22 +271,22 @@ Proof.
   - move => [??] [] ?. lia.
 Qed.
 
-Lemma val_to_Z_unsigned_nonneg v z it :
+Lemma val_to_Z_unsigned_nonneg v z it α :
   it.(it_signed) = false →
-  val_to_Z v it = Some z →
+  val_to_Z v it = Some (α, z) →
   (0 ≤ z)%Z.
 Proof.
   rewrite /val_to_Z.
   case_bool_decide; last done.
   intros Hs Hv.
-  apply bind_Some in Hv as (z' & Hz & Ha).
+  apply bind_Some in Hv as ([? z'] & Hz & Ha).
   apply val_to_Z_go_in_range in Hz.
   rewrite Hs in Ha. simpl in Ha. simplify_eq.
   lia.
 Qed.
 
-Lemma val_to_of_Z z it v p:
-  val_of_Z z it p = Some v → val_to_Z v it = Some z.
+Lemma val_to_of_Z z it v p α :
+  val_of_Z z it p α = Some v → val_to_Z v it = Some (α, z).
 Proof.
   rewrite /val_of_Z /val_to_Z => Ht.
   destruct (bool_decide (z ∈ it)) eqn: Hr => //. simplify_eq.
@@ -271,13 +294,15 @@ Proof.
   have Hlen := bytes_per_int_gt_0 it.
   rewrite /max_int in HM. rewrite /min_int in Hm.
   rewrite val_of_Z_go_length val_to_of_Z_go /=.
-  - case_bool_decide as H => //. clear H.
+  - case_bool_decide as Ha => //. clear Ha.
     destruct (it_signed it) eqn:Hs => /=.
     + case_decide => /=; last (rewrite bool_decide_false //; lia).
-      rewrite bool_decide_true; [f_equal; lia|].
+      rewrite bool_decide_true.
+      { f_equal; f_equal; lia. }
       rewrite int_modulus_twice_half_modulus. move: Hm HM.
       generalize (int_half_modulus it). move => n Hm HM. lia.
     + rewrite bool_decide_false //. lia.
+  - lia. 
   - case_bool_decide as Hneg; case_match; split; try lia.
     + rewrite int_modulus_twice_half_modulus. lia.
     + rewrite /int_modulus /bits_per_int. lia.
@@ -288,9 +313,9 @@ Proof.
     + rewrite /int_modulus /bits_per_int in HM. lia.
 Qed.
 
-Lemma val_of_Z_go_to_prov z n p :
+Lemma val_of_Z_go_to_prov z n p α :
   n ≠ 0%nat →
-  val_to_byte_prov (val_of_Z_go z n p) = p.
+  val_to_byte_prov (val_of_Z_go z n p α) = p.
 Proof.
   destruct n as [|n] => // _. destruct p as [a|] => //.
   rewrite /val_to_byte_prov/=. case_option_guard as Hf => //.
@@ -299,16 +324,16 @@ Proof.
   elim: n z => /=; eauto.
 Qed.
 
-Lemma val_of_Z_to_prov z it p v :
-  val_of_Z z it p = Some v →
+Lemma val_of_Z_to_prov z it p v α :
+  val_of_Z z it p α = Some v →
   val_to_byte_prov v = p.
 Proof.
   rewrite /val_of_Z. case_bool_decide => // -[<-]. apply val_of_Z_go_to_prov.
   have := bytes_per_int_gt_0 it. lia.
 Qed.
 
-Lemma val_to_Z_val_of_loc_n_None n l it:
-  val_to_Z (val_of_loc_n n l) it = None.
+Lemma val_to_Z_val_of_loc_n_None n l it α :
+  val_to_Z (val_of_loc_n n α l) it = None.
 Proof.
   destruct n as [|n].
   - rewrite /val_of_loc_n /= /val_to_Z bool_decide_false //=.
@@ -317,84 +342,103 @@ Proof.
     by case_bool_decide.
 Qed.
 
-Lemma val_to_Z_val_of_loc_None l it:
-  val_to_Z (val_of_loc l) it = None.
+Lemma val_to_Z_val_of_loc_None l it α :
+  val_to_Z (val_of_loc α l) it = None.
 Proof. apply val_to_Z_val_of_loc_n_None. Qed.
 
-Lemma val_to_loc_to_Z_overlap v l it z:
-  val_to_loc v = Some l →
-  val_to_Z v it = Some z →
-  v = NULL_bytes.
-Proof. move => /val_of_to_loc[->|[-> ?//]]. by rewrite val_to_Z_val_of_loc_None. Qed.
+Lemma val_to_Z_NULL_bytes_n it n α : 
+  bytes_per_int it = n →
+  val_to_Z (NULL_bytes_n α n) it = Some (α, 0).
+Proof.
+  intros <-.
+Admitted.
+Lemma val_to_Z_NULL_bytes it α : 
+  bytes_per_int it = bytes_per_addr →
+  val_to_Z (NULL_bytes α) it = Some (α, 0).
+Proof. apply val_to_Z_NULL_bytes_n. Qed.
 
-Lemma val_of_Z_bool_is_Some p it b:
-  is_Some (val_of_Z (bool_to_Z b) it p).
+Lemma val_to_loc_to_Z_overlap v l it z α α' :
+  val_to_loc v = Some (α, l) →
+  val_to_Z v it = Some (α', z) →
+  v = NULL_bytes α ∧ α' = α.
+Proof. 
+  move => /val_of_to_loc[->|[-> ?//]]. 
+  - by rewrite val_to_Z_val_of_loc_None. 
+  - subst. intros Hz.
+    efeed pose proof val_to_Z_length as Hlen; first apply Hz.
+    rewrite val_to_Z_NULL_bytes in Hz; last done.
+    injection Hz as <- <-. done.
+Qed.
+
+Lemma val_of_Z_bool_is_Some p it b α:
+  is_Some (val_of_Z (bool_to_Z b) it p α).
 Proof. apply: val_of_Z_is_Some. apply: bool_to_Z_elem_of_int_type. Qed.
 
-Lemma val_of_Z_bool b it:
-  val_of_Z (bool_to_Z b) it None = Some (i2v (bool_to_Z b) it).
-Proof. rewrite /i2v. by have [? ->]:= val_of_Z_bool_is_Some None it b. Qed.
+Lemma val_of_Z_bool b it α :
+  val_of_Z (bool_to_Z b) it None α = Some (i2v (bool_to_Z b) it α).
+Proof. rewrite /i2v. by have [? ->]:= val_of_Z_bool_is_Some None it b α. Qed.
 
-Program Definition val_of_bool (b : bool) : val :=
-  [MByte (Byte (bool_to_Z b) _) None].
+Program Definition val_of_bool (b : bool) (α : slevel) : val :=
+  [MByte (Byte (bool_to_Z b) _) None α].
 Next Obligation. by destruct b. Qed.
 
-Definition val_to_bool (v : val) : option bool :=
+Definition val_to_bool (v : val) : option (slevel * bool) :=
   match v with
-  | [MByte (Byte 0 _) _] => Some false
-  | [MByte (Byte 1 _) _] => Some true
+  | [MByte (Byte 0 _) _ α] => Some (α, false)
+  | [MByte (Byte 1 _) _ α] => Some (α, true)
   | _                    => None
   end.
 
-Lemma val_to_of_bool b :
-  val_to_bool (val_of_bool b) = Some b.
+Lemma val_to_of_bool b α :
+  val_to_bool (val_of_bool b α) = Some (α, b).
 Proof. by destruct b. Qed.
 
-Lemma val_to_bool_length v b:
-  val_to_bool v = Some b → length v = 1%nat.
+Lemma val_to_bool_length v b α :
+  val_to_bool v = Some (α, b) → length v = 1%nat.
 Proof.
   rewrite /val_to_bool. repeat case_match => //.
 Qed.
 
-Lemma val_to_bool_iff_val_to_Z v b:
-  val_to_bool v = Some b ↔ val_to_Z v u8 = Some (bool_to_Z b).
+Lemma val_to_bool_iff_val_to_Z v b α :
+  val_to_bool v = Some (α, b) ↔ val_to_Z v u8 = Some (α, bool_to_Z b).
 Proof.
   split.
-  - destruct v as [|mb []] => //=; repeat case_match => //=; by move => [<-].
-  - destruct v as [|mb []] => //=; repeat case_match => //=; destruct b => //.
+  - destruct v as [|mb []] => //=; repeat case_match => //=;
+      move => [<- <-]; rewrite /val_to_Z /= slevel_bot_neutral_r//.
+  - destruct v as [|mb []] => //=; repeat case_match => //=; destruct b => //; rewrite /val_to_Z /= slevel_bot_neutral_r//; move => [] <-//.
 Qed.
 
-Lemma val_of_bool_iff_val_of_Z v b:
-  val_of_bool b = v ↔ val_of_Z (bool_to_Z b) u8 None = Some v.
+Lemma val_of_bool_iff_val_of_Z v b α :
+  val_of_bool b α = v ↔ val_of_Z (bool_to_Z b) u8 None α = Some v.
 Proof.
   split.
   - move => <-. destruct b; cbv; do 3 f_equal; by apply byte_eq.
   - destruct b; cbv; move => [<-]; do 2 f_equal; by apply byte_eq.
 Qed.
 
-Lemma i2v_bool_Some b it:
-  val_to_Z (i2v (bool_to_Z b) it) it = Some (bool_to_Z b).
+Lemma i2v_bool_Some b it α :
+  val_to_Z (i2v (bool_to_Z b) it α) it = Some (α, bool_to_Z b).
 Proof. apply: val_to_of_Z. apply val_of_Z_bool. Qed.
 
-Lemma val_of_bool_i2v b :
-  val_of_bool b = i2v (bool_to_Z b) u8.
+Lemma val_of_bool_i2v b α :
+  val_of_bool b α = i2v (bool_to_Z b) u8 α.
 Proof.
   apply val_of_bool_iff_val_of_Z.
   apply val_of_Z_bool.
 Qed.
 
-Definition val_to_Z_ot (v : val) (ot : op_type) : option Z :=
+Definition val_to_Z_ot (v : val) (ot : op_type) : option (slevel * Z) :=
   match ot with
   | IntOp it => val_to_Z v it
-  | BoolOp => bool_to_Z <$> val_to_bool v
+  | BoolOp => (λ '(α, b), (α, bool_to_Z b)) <$> val_to_bool v
   | _ => None
   end.
 
-Lemma val_to_Z_ot_length v ot z:
-  val_to_Z_ot v ot = Some z → length v = (ot_layout ot).(ly_size).
+Lemma val_to_Z_ot_length v ot z α :
+  val_to_Z_ot v ot = Some (α, z) → length v = (ot_layout ot).(ly_size).
 Proof.
   destruct ot => //=.
-  - by move => /fmap_Some[?[/val_to_bool_length -> ?]].
+  - by move => /fmap_Some => [] [[? ?]][/val_to_bool_length -> ?].
   - by move => /val_to_Z_length ->.
 Qed.
 
