theories/caesium/security.v
@@ -1,0 +1,202 @@
+From caesium Require Export base.
+
+Class ConfidentialInterface := {
+  slevel : Set;
+  slevel_eqdec :: EqDecision slevel;
+  slevel_countable :: Countable slevel;
+
+  slevel_bot :: Bottom slevel;
+  slevel_top :: Top slevel;
+  slevel_meet :: Meet slevel;
+  slevel_join :: Join slevel;
+
+  slevel_le :: SqSubsetEq slevel;
+  slevel_preorder :: PreOrder slevel_le;
+
+  slevel_join_ge (s1 s2 : slevel) : slevel_le s1 (s1 ⊔ s2);
+  slevel_meet_le (s1 s2 : slevel) : slevel_le (s1 ⊓ s2) s1;
+
+  slevel_top_max (s : slevel) : slevel_le s ⊤;
+  slevel_bot_min (s : slevel) : slevel_le ⊥ s;
+
+  slevel_meet_idemp (s : slevel) : s ⊓ s = s;
+  slevel_join_idemp (s : slevel) : s ⊔ s = s;
+  slevel_join_comm : Comm (=) (slevel_join);
+  slevel_meet_comm : Comm (=) (slevel_meet);
+
+  slevel_bot_neutral_r (s : slevel) : s ⊔ ⊥ = s;
+  slevel_top_neutral_r (s : slevel) : s ⊓ ⊤ = s;
+}.
+Global Instance inhabited_slevel `{!ConfidentialInterface}: Inhabited slevel := populate slevel_bot.
+
+(** We can define one particular lattice over a set of principals in the following way: *)
+Class Principals := {
+  principals : Set;
+  principals_eqdec :: EqDecision principals;
+  principals_countable :: Countable principals;
+}.
+Section flow_tracking.
+  Context `{Principals}.
+
+  Inductive principal_set :=
+    | AllPrincipals
+    | SetOfPrincipals (p : gset principals).
+  Global Instance principal_set_eqdec : EqDecision principal_set.
+  Proof. solve_decision. Defined.
+  Global Instance principal_set_countable : Countable principal_set.
+  Proof.
+  Admitted.
+  Global Instance principal_set_empty : Empty principal_set := SetOfPrincipals ∅.
+  Global Instance principal_set_intersection : Intersection principal_set :=
+    λ ps1 ps2,
+      match ps1, ps2 with
+      | AllPrincipals, AllPrincipals => AllPrincipals
+      | SetOfPrincipals s1, AllPrincipals => SetOfPrincipals s1
+      | SetOfPrincipals s1, SetOfPrincipals s2 => SetOfPrincipals (s1 ∩ s2)
+      | AllPrincipals, SetOfPrincipals s2 => SetOfPrincipals s2
+      end.
+  Global Instance principal_set_union : Union principal_set :=
+    λ ps1 ps2,
+      match ps1, ps2 with
+      | AllPrincipals, AllPrincipals => AllPrincipals
+      | SetOfPrincipals s1, AllPrincipals => AllPrincipals
+      | SetOfPrincipals s1, SetOfPrincipals s2 => SetOfPrincipals (s1 ∪ s2)
+      | AllPrincipals, SetOfPrincipals s2 => AllPrincipals
+      end.
+  Global Instance principal_set_subseteq : SubsetEq principal_set :=
+    λ ps1 ps2,
+      match ps1, ps2 with
+      | AllPrincipals, AllPrincipals => True
+      | SetOfPrincipals s1, AllPrincipals => True
+      | SetOfPrincipals s1, SetOfPrincipals s2 => s1 ⊆ s2
+      | AllPrincipals, SetOfPrincipals s2 => False
+      end.
+  Global Instance principal_set_union_right_id : RightId eq ∅ principal_set_union.
+  Proof. intros []; simpl; first done. f_equiv. set_solver. Qed.
+  Global Instance principal_set_union_left_id : LeftId eq ∅ principal_set_union.
+  Proof. intros []; simpl; first done. f_equiv. set_solver. Qed.
+  Global Instance principal_set_intersection_right_id : RightId eq AllPrincipals principal_set_intersection.
+  Proof. intros []; simpl; done. Qed.
+  Global Instance principal_set_intersection_left_id : LeftId eq AllPrincipals principal_set_intersection.
+  Proof. intros []; simpl; done. Qed.
+
+  Global Instance principal_set_preorder : PreOrder principal_set_subseteq.
+  Proof.
+    constructor.
+    - intros []; rewrite /subseteq/principal_set_subseteq; simpl; set_solver.
+    - intros [][][]; rewrite /subseteq/principal_set_subseteq; simpl; set_solver.
+  Qed.
+
+  (* Two lattices, integrity and confidentiality. sources and readers. *)
+  Record conf_policy := mk_policy {
+    conf_readers : principal_set;
+    conf_sources : principal_set;
+  }.
+  Instance conf_policy_eqdec : EqDecision conf_policy.
+  Proof. solve_decision. Defined.
+  Instance conf_policy_countable : Countable conf_policy.
+  Proof.
+  Admitted.
+
+  Instance conf_bot : Bottom conf_policy := mk_policy AllPrincipals ∅.
+  Instance conf_top : Top conf_policy := mk_policy ∅ AllPrincipals.
+  Instance: Inhabited conf_policy := populate ⊥.
+
+  Instance conf_join : Join conf_policy :=
+    λ (s1 s2 : conf_policy), {|
+      conf_readers := s1.(conf_readers) ∩ s2.(conf_readers);
+      conf_sources := s1.(conf_sources) ∪ s2.(conf_sources);
+    |}.
+  Instance conf_meet : Meet conf_policy :=
+    λ (s1 s2 : conf_policy), {|
+      conf_readers := s1.(conf_readers) ∪ s2.(conf_readers);
+      conf_sources := s1.(conf_sources) ∩ s2.(conf_sources);
+    |}.
+
+  (* s1 ⊑ s2 holds iff s1 is less restrictive, i.e. s2 upholds all the constraints of s1. *)
+  Instance conf_le : SqSubsetEq conf_policy :=
+    λ s1 s2, s2.(conf_readers) ⊆ s1.(conf_readers) ∧ s1.(conf_sources) ⊆ s2.(conf_sources).
+
+  Instance conf_le_partial_order : PreOrder conf_le.
+  Proof.
+    constructor.
+    - intros [??]; rewrite /conf_le/=; done.
+    - intros [??] [??] [??]; rewrite /conf_le/=; intros [] [];
+      split; etrans; done.
+  Qed.
+
+  (** Declassification is allowed if:
+     - the declassifiers cover all sources of the old policy
+     - OR the set of readers does not grow and the set of sources can only be changed by removing declassifiers or adding additional sources
+   *)
+  Definition allow_declassification_group (declassifiers : principal_set) (from to : conf_policy) :=
+    from.(conf_sources) ⊆ declassifiers ∨
+    (to.(conf_readers) ⊆ from.(conf_readers) ∧ from.(conf_sources) ⊆ to.(conf_sources) ∪ declassifiers).
+  Definition allow_declassification (declassifier : principals) :=
+    allow_declassification_group (SetOfPrincipals {[ declassifier ]}).
+
+  Instance allow_declassification_group_trans declassifiers :
+    Transitive (allow_declassification_group declassifiers).
+  Proof.
+    destruct declassifiers as [];
+    intros [[] []][[] []][[] []];
+    rewrite /allow_declassification_group/=/subseteq/principal_set_subseteq/=;
+    set_solver.
+  Qed.
+  Instance allow_declassification_group_refl declassifiers :
+    Reflexive (allow_declassification_group declassifiers).
+  Proof.
+    destruct declassifiers as [];
+    intros [[] []];
+    rewrite /allow_declassification_group/=/subseteq/principal_set_subseteq/=;
+    set_solver.
+  Qed.
+
+  (** We can get a simple declassification operation that has a neutral element by expanding the existing policy to allow a "required" set of readers *)
+  Definition declassify_for (from : conf_policy) (require : conf_policy) : conf_policy :=
+    from ⊓ require.
+  (* This operation has a neutral element *)
+  Lemma declassify_for_neutral declassifiers from :
+    allow_declassification_group declassifiers from (declassify_for from ⊤).
+  Proof.
+    right. simpl. split.
+    - destruct from as [readers sources]; simpl. rewrite right_id//.
+    - rewrite right_id.
+      destruct from as [[][]], declassifiers as []; rewrite /subseteq/principal_set_subseteq/=; set_solver.
+  Qed.
+
+
+  Program Definition flow_tracking_interface : ConfidentialInterface := {|
+    slevel := conf_policy;
+  |}.
+  Solve Obligations with try apply _.
+  Next Obligation.
+  Admitted.
+  Next Obligation.
+  Admitted.
+
+  Next Obligation.
+  Admitted.
+
+  Next Obligation.
+  Admitted.
+
+  Next Obligation.
+  Admitted.
+
+  Next Obligation.
+  Admitted.
+
+  Next Obligation.
+  Admitted.
+
+  Next Obligation.
+  Admitted.
+
+  Next Obligation.
+  Admitted.
+
+  Next Obligation.
+  Admitted.
+
+End flow_tracking.
